theories/Core/ITreeDefinition.v
@@ -210,7 +210,7 @@ Definition map {E R S} (f : R -> S)  (t : itree E R) : itree E S :=
 (** Atomic itrees triggering a single event. *)
 Definition trigger {E : Type -> Type} : E ~> itree E :=
   fun R e => Vis e (fun x => Ret x).
-Instance trigger_itree {E: Type -> Type} : Triggerable (itree E) E := trigger.
+(* Instance trigger_itree {E: Type -> Type} : Triggerable (itree E) E := trigger. *)
 
 (** Ignore the result of a tree. *)
 Definition ignore {E R} : itree E R -> itree E unit :=
